

# Group assignment 2

Assignment 2.21

November 2025

## **Group Members**

Baraa Magdy

Celia Medina Giménez

Dino Keylas

Maria Naz

Oskar Johannes Piibar

## Problem 1.

We assume the conditional distribution

$$Y \mid X = x \sim \text{Poisson}(\lambda(x)), \quad \lambda(x) = \exp(\alpha \cdot x + \beta),$$

where  $\alpha \in \mathbb{R}^p$  is a slope vector and  $\beta \in \mathbb{R}$  is an intercept. The conditional pmf for a single observation  $(x, y)$  is

$$f_{Y|X}(y \mid x) = \frac{\lambda(x)^y e^{-\lambda(x)}}{y!}.$$

Following the Maximum Likelihood viewpoint (Section 4.2.1: Maximum Likelihood and regression), derive the loss to be minimized w.r.t.  $\alpha, \beta$ . Address whether the factorial term is needed.

### Log-likelihood and negative log-likelihood

For one observation  $(x, y)$  the log-likelihood is

$$\ell(\alpha, \beta \mid x, y) = \log f_{Y|X}(y \mid x) = y \log \lambda(x) - \lambda(x) - \log(y!).$$

Using  $\log \lambda(x) = \alpha \cdot x + \beta$  and  $\lambda(x) = \exp(\alpha \cdot x + \beta)$  we get

$$\ell(\alpha, \beta \mid x, y) = y(\alpha \cdot x + \beta) - \exp(\alpha \cdot x + \beta) - \log(y!).$$

The negative log-likelihood (loss) for a single observation is therefore

$$\ell_{\text{neg}}(\alpha, \beta \mid x, y) = -y(\alpha \cdot x + \beta) + \exp(\alpha \cdot x + \beta) + \log(y!).$$

For a dataset  $\{(x_i, y_i)\}_{i=1}^n$  the total negative log-likelihood is

$$L(\alpha, \beta) = \sum_{i=1}^n [-y_i(\alpha \cdot x_i + \beta) + \exp(\alpha \cdot x_i + \beta) + \log(y_i!)].$$

### Practical loss to minimize

The term  $\sum_{i=1}^n \log(y_i!)$  does *not* depend on the parameters  $(\alpha, \beta)$ . Hence it is a constant for optimization and can be dropped. The practical loss (negative log-likelihood up to an additive constant) to minimize is

$$\tilde{L}(\alpha, \beta) = \sum_{i=1}^n [\exp(\alpha \cdot x_i + \beta) - y_i(\alpha \cdot x_i + \beta)].$$

Thus *we do not need the factorial term* when performing parameter estimation by MLE, because it does not affect the location of the minimizer.

### Score (first-order) equations

Define  $\lambda_i = \exp(\alpha \cdot x_i + \beta)$ . The gradient (score) components are

$$\frac{\partial \tilde{L}}{\partial \alpha} = \sum_{i=1}^n (\lambda_i - y_i) x_i, \quad \frac{\partial \tilde{L}}{\partial \beta} = \sum_{i=1}^n (\lambda_i - y_i).$$

Setting these to zero yields the likelihood equations

$$\sum_{i=1}^n (\lambda_i - y_i) x_i = 0, \quad \sum_{i=1}^n (\lambda_i - y_i) = 0,$$

which are the analogues of the normal equations for Poisson regression.

### Hessian and convexity

Second derivatives give the Hessian blocks

$$\frac{\partial^2 \tilde{L}}{\partial \alpha \partial \alpha^\top} = \sum_{i=1}^n \lambda_i x_i x_i^\top, \quad \frac{\partial^2 \tilde{L}}{\partial \beta^2} = \sum_{i=1}^n \lambda_i, \quad \frac{\partial^2 \tilde{L}}{\partial \alpha \partial \beta} = \sum_{i=1}^n \lambda_i x_i.$$

Since  $\lambda_i > 0$  for all  $i$ , the Hessian is positive semidefinite (in typical cases positive definite), so  $\tilde{L}$  is convex in  $(\alpha, \beta)$  and standard convex optimization methods apply.

### Connection to GLM / IRLS

Minimizing  $\tilde{L}$  is exactly maximum likelihood estimation for a Generalized Linear Model with Poisson family and log link. Typical solvers use Newton / Fisher scoring / IRLS (iteratively reweighted least squares), where in each iteration weights proportional to  $\lambda_i$  appear.

### Summary (final answer)

The loss to minimize (negative log-likelihood up to constant) is

$$\tilde{L}(\alpha, \beta) = \sum_{i=1}^n \left[ \exp(\alpha \cdot x_i + \beta) - y_i(\alpha \cdot x_i + \beta) \right].$$

The factorial term  $\log(y_i!)$  can be omitted during optimization because it does not depend on  $(\alpha, \beta)$ .

## Problem 2.

Let  $X_1, X_2, \dots, X_n$  be i.i.d. random variables from  $\text{Uniform}(0, \theta)$ .

Let  $\hat{\theta} = \max(X_1, X_2, \dots, X_n)$ .

(a) Find the distribution function of  $\hat{\theta}$ .

(b) Compute the bias  $\text{Bias}(\hat{\theta})$ , the standard error  $\text{SE}(\hat{\theta})$ , and the mean squared error  $\text{MSE}(\hat{\theta})$ .

### Problem 2a.

#### CDF of $\hat{\theta}$

We want CDF of

$$\hat{\theta} = \max(X_1, X_2, \dots, X_n)$$

That means we need

$$F_{\hat{\theta}}(x) = P(\hat{\theta} \leq x)$$

If the maximum ( $\hat{\theta}$ ) is  $\leq x$ , that means

$$\max(X_1, X_2, \dots, X_n) \leq x$$

Hence,

$$P(\hat{\theta} \leq x) = P(X_1 \leq x, X_2 \leq x, \dots, X_n \leq x)$$

Because  $X_i$ 's are independent, then

$$P(X_1 \leq x, X_2 \leq x, \dots, X_n \leq x) = P(X_1 \leq x) \cdot P(X_2 \leq x) \cdot \dots P(X_n \leq x)$$

Since each has the same CDF,  $F_X(x)$ , this becomes

$$P(\hat{\theta} \leq x) = [F_X(x)]^n$$

For a  $\text{Uniform}(0, \theta)$  random variables:

$$F_X(x) = \begin{cases} 0, & x < 0, \\ \left(\frac{x}{\theta}\right), & 0 \leq x \leq \theta, \\ 1, & x > \theta. \end{cases}$$

As We know that  $P(\hat{\theta} \leq x) = [F_X(x)]^n$ , then the **CDF** of  $\hat{\theta}$ :

$$F_{\hat{\theta}}(x) = \begin{cases} 0, & x < 0, \\ \left(\frac{x}{\theta}\right)^n, & 0 \leq x \leq \theta, \\ 1, & x > \theta. \end{cases}$$

By differentiating the **CDF**, we can get the **PDF**:

$$\begin{aligned} f_{\hat{\theta}}(x) &= \frac{d}{dx} F_{\hat{\theta}}(x) \\ &= \frac{d}{dx} \left(\frac{x}{\theta}\right)^n \\ &= \frac{n}{\theta^n} x^{n-1}, \quad 0 \leq x \leq \theta \end{aligned}$$

**Problem 2b.****Bias:**

$$\text{Bias}(\hat{\theta}) = E(\hat{\theta}) - \theta$$

Calculate  $E(\hat{\theta})$ :

$$\begin{aligned} E(\hat{\theta}) &= \int_0^\theta x f(x) dx = \int_0^\theta x \cdot \frac{n}{\theta^n} x^{n-1} dx = \frac{n}{\theta^n} \int_0^\theta x^n dx \\ &= \frac{n}{\theta^n} \cdot \frac{\theta^{n+1}}{n+1} = \frac{n}{n+1} \theta. \end{aligned}$$

Plug  $E(\hat{\theta})$  to the bias formula:

$$\text{Bias}(\hat{\theta}) = E(\hat{\theta}) - \theta = \frac{n}{n+1} \theta - \theta = -\frac{1}{n+1} \theta.$$

**Standard Error:**

$$\text{SE}(\hat{\theta}) = \sqrt{\text{Var}(\hat{\theta})}$$

Calculate  $\text{Var}(\hat{\theta})$ :

$$\begin{aligned} E(\hat{\theta}^2) &= \int_0^\theta x^2 f(x) dx = \frac{n}{\theta^n} \int_0^\theta x^{n+1} dx = \frac{n}{\theta^n} \cdot \frac{\theta^{n+2}}{n+2} = \frac{n}{n+2} \theta^2. \\ \text{Var}(\hat{\theta}) &= E(\hat{\theta}^2) - [E(\hat{\theta})]^2 = \frac{n}{n+2} \theta^2 - \left( \frac{n}{n+1} \theta \right)^2 \\ &= \theta^2 \left( \frac{n}{n+2} - \frac{n^2}{(n+1)^2} \right) = \theta^2 \cdot \frac{n}{(n+2)(n+1)^2}. \end{aligned}$$

Plug  $\text{Var}(\hat{\theta})$  to the SE formula:

$$\text{SE}(\hat{\theta}) = \sqrt{\text{Var}(\hat{\theta})} = \theta \sqrt{\frac{n}{(n+2)(n+1)^2}} = \frac{\theta}{n+1} \sqrt{\frac{n}{n+2}}.$$

**Mean Squared Error:**

$$\begin{aligned} \text{MSE}(\hat{\theta}) &= \text{Bias}(\hat{\theta})^2 + \text{Var}(\hat{\theta}) \\ &= \left( -\frac{\theta}{n+1} \right)^2 + \frac{n \theta^2}{(n+1)^2(n+2)} \\ &= \frac{\theta^2}{(n+1)^2} + \frac{n \theta^2}{(n+1)^2(n+2)} \\ &= \frac{\theta^2}{(n+1)^2} \left( 1 + \frac{n}{n+2} \right) \\ &= \frac{\theta^2}{(n+1)^2} \cdot \frac{n+2+n}{n+2} \\ &= \frac{(n+3) \theta^2}{(n+1)^2(n+2)}. \end{aligned}$$

**Problem 3.**

Consider the continuous distribution with density

$$p(x) = \frac{1}{2} \cos x, \quad -\frac{\pi}{2} < x < \frac{\pi}{2},$$

**Problem 3a.**

Find the distribution function  $F(x)$

**Solution**

By definition,

$$F(x) = \int_{-\infty}^x f(v) dv.$$

When  $x \leq -\frac{\pi}{2} \Rightarrow F(x) = 0$ , and when  $x \geq \frac{\pi}{2} \Rightarrow F(x) = 1$ .

Otherwise,

$$F(x) = \int_{-\pi/2}^x \frac{1}{2} \cos(t) dt = \frac{1}{2} [\sin(t)]_{-\pi/2}^x = \frac{1}{2} (\sin(x) + 1).$$

So,

$$F(x) = \begin{cases} 0, & x \leq -\frac{\pi}{2}, \\ \frac{1}{2} (\sin(x) + 1), & -\frac{\pi}{2} < x < \frac{\pi}{2}, \\ 1, & x \geq \frac{\pi}{2}. \end{cases}$$

**Problem 3b.**

Find the inverse distribution function  $F^{-1}(u)$

**Solution**

From part (a),

$$F(x) = \frac{1}{2} (\sin(x) + 1).$$

So we set

$$u = F(x) = \frac{1}{2} (\sin(x) + 1)$$

Now, let's just solve for x.

$$2u - 1 = \sin(x) \Rightarrow x = \arcsin(2u - 1).$$

Therefore,

$$F^{-1}(u) = \arcsin(2u - 1), \quad 0 < u < 1.$$

**Problem 3c.**

To sample using an *Accept-Reject sampler* (Algorithm 1), we need to find a density  $g(x)$  such that

$$p(x) \leq M g(x) \quad \text{for some } M > 0.$$

Find such a density  $g$  and determine the corresponding value of  $M$ .

### Solution

$p(x)$  is bounded and has an "easy" shape (symmetric, has a maximum at  $x=0$ , and goes to 0 at its boundaries). This means a uniform distribution on the same interval seems appropriate. So let  $g(x)$ :

$$g(x) = \frac{1}{b-a} = \frac{1}{\pi}, \quad x \in \left[-\frac{\pi}{2}, \frac{\pi}{2}\right].$$

Now, let's check that it is a valid pdf:

$$\int_a^b g(x) dx = \int_{-\pi/2}^{\pi/2} \frac{1}{\pi} dx = \frac{1}{\pi}(\pi) = 1.$$

Hence,  $g(x)$  is a valid pdf.

We require that  $p(x) \leq Mg(x)$  for all  $x$ .

$$\frac{p(x)}{g(x)} \leq M \Rightarrow \frac{p(x)}{g(x)} = \frac{\frac{1}{2} \cos(x)}{\frac{1}{\pi}} = \frac{\pi}{2} \cos(x)$$

We look for the maximum of  $\frac{p(x)}{g(x)}$  at  $x = 0$  to find the lowest value of  $M$  that would "cover" all  $p(x)$  with  $g(x)M$ .

$$M = \frac{\pi}{2} \cos(0) = \frac{\pi}{2}.$$

Thus:

$$M = \frac{\pi}{2}, \quad g(x) = \frac{1}{\pi}.$$

This makes sense graphically, since  $Mg(x)$  just covers  $p(x)$  at its maximum.

#### Problem 4.

Let  $Y_1, Y_2, \dots, Y_n$  be a sequence of IID discrete random variables, where  $P(Y_i = 0) = 0.1$ ,  $P(Y_i = 1) = 0.3$ ,  $P(Y_i = 2) = 0.2$ , and  $P(Y_i = 3) = 0.4$ . Let  $X_n = \max\{Y_1, Y_2, \dots, Y_n\}$ . Let  $X_0 = 0$  and verify that  $(X_0, X_1, \dots, X_n)$  is a Markov chain. Find the transition matrix  $P$ .

#### Solution

To show that  $(X_0, X_1, \dots, X_n)$  is a Markov chain, we have to prove that it has at most 1-step memory.

For a step  $X_n$  in the chain, we can say that:

$$\mathbb{P}(X_n = x_n \mid X_{n-1} = x_{n-1}, X_{n-2} = x_{n-2}, \dots, X_0 = x_0).$$

From the problem definition, we know that  $X_n$  is the maximum of all the previous Y's:

$$X_n = \max\{Y_1, Y_2, \dots, Y_n\},$$

which can be rewritten as

$$\max\{X_{n-1}, Y_n\},$$

because

$$(X_1, X_2, \dots, X_{n-1}) = (X_1 = \max\{Y_1\}, X_2 = \max\{Y_1, Y_2\}, \dots, \\ X_{n-2} = \max\{Y_1, Y_2, \dots, Y_{n-2}\}, X_{n-1} = \max\{Y_1, Y_2, \dots, Y_{n-1}\}).$$

Now, rewriting the initial statement gives us:

$$\mathbb{P}(\max\{X_{n-1}, Y_n\} = x_n \mid \max\{X_{n-2}, Y_{n-1}\} = x_{n-1}, \max\{X_{n-3}, Y_{n-2}\} = x_{n-2}, \dots, \max\{X_0, Y_1\} = x_1, X_0 = x_0).$$

However, since the sequence of Y's is independent, this means that  $Y_n$  is independent of previous  $(Y_1, Y_2, \dots, Y_{n-1})$  and also independent of  $(X_1, X_2, \dots, X_{n-1})$ . Therefore, conditioning on earlier X's beyond  $X_{n-1}$  does not affect the distribution of  $X_n$ . Taking this into account, we can write the last statement as:

$$\begin{aligned} \mathbb{P}(\max\{X_{n-1}, Y_n\} = x_n \mid \max\{X_{n-2}, Y_{n-1}\} = x_{n-1}, \max\{X_{n-3}, Y_{n-2}\} = x_{n-2}, \dots, \max\{X_0, Y_1\} = x_1, X_0 = x_0) \\ = \mathbb{P}(\max\{X_{n-1}, Y_n\} = x_n \mid \max\{X_{n-2}, Y_{n-1}\} = x_{n-1}) \\ = \mathbb{P}(X_n = x_n \mid X_{n-1} = x_{n-1}), \end{aligned}$$

which is the definition of being a Markov chain. This concludes verifying that  $(X_0, X_1, \dots, X_n)$  is a Markov chain.

To construct the transition matrix  $P$  we begin by identifying the dimensions of the matrix. As  $Y$  can take 4 different values -  $\{0, 1, 2, 3\}$  - the matrix will be a 4x4 matrix. This is because we have 4 states to begin from (the rows) and 4 states to go to (the columns).

Now to fill it with values the following logic was applied: for each entry  $P_{ij}$  in matrix  $P$ , where  $i$  indicates the row and  $j$  the column, both in the range (0-3), conditional probability was applied. For example, the row  $P_{00}, P_{01}, P_{02}, P_{03}$  was filled out with the probabilities given in the exercise, which indicates going from state  $X_{n-1} = 0$  to  $X_n = 0, 1, 2, 3$ , respectively. Let us assume that we are now at state  $X_n = 1$  and as  $X_{n+1} = \max\{X_n, Y_{n+1}\}$  then returning to state 0 is no longer possible ( $P_{10} = 0$ ). Now  $P_{11}$  equals the probability that  $Y_i = 0$  or  $Y_i = 1 \Rightarrow 0.1 + 0.3 = 0.4$ .  $P_{12}$  and  $P_{13}$  are filled in a similar way to the fields  $P_{02}, P_{03}$ . For the row vector  $P_{20}, P_{21}, P_{22}, P_{23}$ , we can no longer reach the states 0, 1, therefore  $P_{20}, P_{21} = 0$  and  $P_{22} = \mathbb{P}(Y_i = 0) + \mathbb{P}(Y_i = 1) + \mathbb{P}(Y_i = 2) = 0.1 + 0.3 + 0.2 = 0.6$ . Reaching state 3 from initial state 2 has a probability of 0.4, given in the exercise description. For the final row vector  $P_{30}, P_{31}, P_{32}, P_{33}$ , we can no longer reach any of the states other than 3, therefore  $P_{30}, P_{31}, P_{32} = 0$  and  $P_{33} = 0.1 + 0.3 + 0.2 + 0.4 = 1$ . The completed transition matrix  $P$  can be seen below:



$$P = \begin{matrix} & \begin{matrix} 0 & 1 & 2 & 3 \end{matrix} \\ \begin{matrix} 0 \\ 1 \\ 2 \\ 3 \end{matrix} & \begin{pmatrix} 0.1 & 0.3 & 0.2 & 0.4 \\ 0 & 0.4 & 0.2 & 0.4 \\ 0 & 0 & 0.6 & 0.4 \\ 0 & 0 & 0 & 1 \end{pmatrix} \end{matrix}.$$

The rows of a transition matrix have to sum up to 1, which is the case for the constructed matrix, giving reasons to believe that it was filled properly.

**Problem 5.**

Let  $X_1, \dots, X_n$  be IID from an unknown distribution  $F$ . Let  $\hat{F}_n$  be the empirical distribution function. Use this to find an estimate of the  $p$ -quantile of  $F$  (call it  $q$ ). Use Theorem 5.28 to find a confidence interval for  $q$ .

**Solution.**

Let  $X_1, \dots, X_n \stackrel{\text{iid}}{\sim} F$  with empirical CDF

$$\hat{F}_n(x) = \frac{1}{n} \sum_{i=1}^n \mathbf{1}\{X_i \leq x\}, \quad X_{(1)} \leq \dots \leq X_{(n)} \text{ (order statistics).}$$

For a fixed  $p \in (0, 1)$  the population  $p$ -quantile (Remark 6.15) is:

$$q_p := F^{-1}(p) = \inf\{x : F(x) \geq p\}.$$

The empirical  $p$ -quantile is the inverse of  $\hat{F}_n$ :

$$\hat{q}_p := \hat{F}_n^{-1}(p) = X_{(\lceil np \rceil)}.$$

Here  $np$  is the product of the sample size  $n$  and the probability level  $p$ ; it is the expected rank (i.e., the expected number of observations  $\leq q_p$ ) in a sample of size  $n$ . Taking  $\lceil np \rceil$  chooses the smallest index whose cumulative proportion  $k/n$  is at least  $p$ .

**Confidence interval via DKW (Theorem 5.28).**

The Dvoretzky–Kiefer–Wolfowitz inequality says that for any  $\varepsilon > 0$ ,

$$\Pr\left(\sup_x |\hat{F}_n(x) - F(x)| > \varepsilon\right) \leq 2e^{-2n\varepsilon^2}.$$

For a confidence level  $1 - \alpha$ , set

$$\varepsilon_\alpha := \sqrt{\frac{1}{2n} \log \frac{2}{\alpha}}.$$

Then, with probability at least  $1 - \alpha$ ,

$$q_p \in [\hat{F}_n^{-1}(p - \varepsilon_\alpha), \hat{F}_n^{-1}(p + \varepsilon_\alpha)].$$

Since  $\hat{F}_n^{-1}(u) = X_{(\lceil nu \rceil)}$ , this becomes the explicit interval

$$\text{CI}_{1-\alpha}(q_p) = \left[ X_{(\lceil n \underline{p} \rceil)}, X_{(\lceil n \bar{p} \rceil)} \right], \quad \underline{p} = \max\{0, p - \varepsilon_\alpha\}, \quad \bar{p} = \min\{1, p + \varepsilon_\alpha\}.$$